misc tuning and modernization;

src/HOL/Algebra/More_Group.thy
@@ -5,8 +5,7 @@
 section \<open>More on groups\<close>
 
 theory More_Group
-imports
-  Ring
+  imports Ring
 begin
 
 text \<open>
@@ -16,63 +15,62 @@ text \<open>
   facts about the unit group within the ring locale.
 \<close>
 
-definition units_of :: "('a, 'b) monoid_scheme => 'a monoid" where
-  "units_of G == (| carrier = Units G,
-     Group.monoid.mult = Group.monoid.mult G,
-     one  = one G |)"
+definition units_of :: "('a, 'b) monoid_scheme \<Rightarrow> 'a monoid"
+  where "units_of G =
+    \<lparr>carrier = Units G, Group.monoid.mult = Group.monoid.mult G, one  = one G\<rparr>"
 
-lemma (in monoid) units_group: "group(units_of G)"
+lemma (in monoid) units_group: "group (units_of G)"
   apply (unfold units_of_def)
   apply (rule groupI)
-  apply auto
-  apply (subst m_assoc)
-  apply auto
+      apply auto
+   apply (subst m_assoc)
+      apply auto
   apply (rule_tac x = "inv x" in bexI)
-  apply auto
+   apply auto
   done
 
-lemma (in comm_monoid) units_comm_group: "comm_group(units_of G)"
+lemma (in comm_monoid) units_comm_group: "comm_group (units_of G)"
   apply (rule group.group_comm_groupI)
-  apply (rule units_group)
+   apply (rule units_group)
   apply (insert comm_monoid_axioms)
   apply (unfold units_of_def Units_def comm_monoid_def comm_monoid_axioms_def)
   apply auto
   done
 
 lemma units_of_carrier: "carrier (units_of G) = Units G"
-  unfolding units_of_def by auto
+  by (auto simp: units_of_def)
 
-lemma units_of_mult: "mult(units_of G) = mult G"
-  unfolding units_of_def by auto
+lemma units_of_mult: "mult (units_of G) = mult G"
+  by (auto simp: units_of_def)
 
-lemma units_of_one: "one(units_of G) = one G"
-  unfolding units_of_def by auto
+lemma units_of_one: "one (units_of G) = one G"
+  by (auto simp: units_of_def)
 
-lemma (in monoid) units_of_inv: "x : Units G ==> m_inv (units_of G) x = m_inv G x"
+lemma (in monoid) units_of_inv: "x \<in> Units G \<Longrightarrow> m_inv (units_of G) x = m_inv G x"
   apply (rule sym)
   apply (subst m_inv_def)
   apply (rule the1_equality)
-  apply (rule ex_ex1I)
-  apply (subst (asm) Units_def)
-  apply auto
-  apply (erule inv_unique)
-  apply auto
-  apply (rule Units_closed)
-  apply (simp_all only: units_of_carrier [symmetric])
-  apply (insert units_group)
-  apply auto
-  apply (subst units_of_mult [symmetric])
-  apply (subst units_of_one [symmetric])
-  apply (erule group.r_inv, assumption)
+   apply (rule ex_ex1I)
+    apply (subst (asm) Units_def)
+    apply auto
+     apply (erule inv_unique)
+        apply auto
+    apply (rule Units_closed)
+    apply (simp_all only: units_of_carrier [symmetric])
+    apply (insert units_group)
+    apply auto
+   apply (subst units_of_mult [symmetric])
+   apply (subst units_of_one [symmetric])
+   apply (erule group.r_inv, assumption)
   apply (subst units_of_mult [symmetric])
   apply (subst units_of_one [symmetric])
   apply (erule group.l_inv, assumption)
   done
 
-lemma (in group) inj_on_const_mult: "a: (carrier G) ==> inj_on (%x. a \<otimes> x) (carrier G)"
+lemma (in group) inj_on_const_mult: "a \<in> carrier G \<Longrightarrow> inj_on (\<lambda>x. a \<otimes> x) (carrier G)"
   unfolding inj_on_def by auto
 
-lemma (in group) surj_const_mult: "a : (carrier G) ==> (%x. a \<otimes> x) ` (carrier G) = (carrier G)"
+lemma (in group) surj_const_mult: "a \<in> carrier G \<Longrightarrow> (\<lambda>x. a \<otimes> x) ` carrier G = carrier G"
   apply (auto simp add: image_def)
   apply (rule_tac x = "(m_inv G a) \<otimes> x" in bexI)
   apply auto
@@ -82,33 +80,29 @@ lemma (in group) surj_const_mult: "a : (carrier G) ==> (%x. a \<otimes> x) ` (ca
   apply auto
   done
 
-lemma (in group) l_cancel_one [simp]:
-    "x : carrier G \<Longrightarrow> a : carrier G \<Longrightarrow> (x \<otimes> a = x) = (a = one G)"
+lemma (in group) l_cancel_one [simp]: "x \<in> carrier G \<Longrightarrow> a \<in> carrier G \<Longrightarrow> x \<otimes> a = x \<longleftrightarrow> a = one G"
   apply auto
   apply (subst l_cancel [symmetric])
-  prefer 4
-  apply (erule ssubst)
-  apply auto
+     prefer 4
+     apply (erule ssubst)
+     apply auto
   done
 
-lemma (in group) r_cancel_one [simp]: "x : carrier G \<Longrightarrow> a : carrier G \<Longrightarrow>
-    (a \<otimes> x = x) = (a = one G)"
+lemma (in group) r_cancel_one [simp]: "x \<in> carrier G \<Longrightarrow> a \<in> carrier G \<Longrightarrow> a \<otimes> x = x \<longleftrightarrow> a = one G"
   apply auto
   apply (subst r_cancel [symmetric])
-  prefer 4
-  apply (erule ssubst)
-  apply auto
+     prefer 4
+     apply (erule ssubst)
+     apply auto
   done
 
 (* Is there a better way to do this? *)
-lemma (in group) l_cancel_one' [simp]: "x : carrier G \<Longrightarrow> a : carrier G \<Longrightarrow>
-    (x = x \<otimes> a) = (a = one G)"
+lemma (in group) l_cancel_one' [simp]: "x \<in> carrier G \<Longrightarrow> a \<in> carrier G \<Longrightarrow> x = x \<otimes> a \<longleftrightarrow> a = one G"
   apply (subst eq_commute)
   apply simp
   done
 
-lemma (in group) r_cancel_one' [simp]: "x : carrier G \<Longrightarrow> a : carrier G \<Longrightarrow>
-    (x = a \<otimes> x) = (a = one G)"
+lemma (in group) r_cancel_one' [simp]: "x \<in> carrier G \<Longrightarrow> a \<in> carrier G \<Longrightarrow> x = a \<otimes> x \<longleftrightarrow> a = one G"
   apply (subst eq_commute)
   apply simp
   done
@@ -118,7 +112,7 @@ lemma (in group) r_cancel_one' [simp]: "x : carrier G \<Longrightarrow> a : carr
 
 lemma (in comm_group) power_order_eq_one:
   assumes fin [simp]: "finite (carrier G)"
-    and a [simp]: "a : carrier G"
+    and a [simp]: "a \<in> carrier G"
   shows "a (^) card(carrier G) = one G"
 proof -
   have "(\<Otimes>x\<in>carrier G. x) = (\<Otimes>x\<in>carrier G. a \<otimes> x)"
